Make query ordType and add eq function for response objects
The ordType for the queries is obtained through isomorphism with GenTree.

The equality for the response objects considers order in the list of
responses in the case of NestedListResult.

src/Query.v
@@ -6,7 +6,11 @@ Unset Printing Implicit Defensive.
 
 From extructures Require Import ord fmap.
 
+Require Import treeordtype.
 Require Import Schema.
+Require Import SchemaAux.
+
+
 
 Section Query.
 
@@ -18,7 +22,7 @@ Section Query.
   | LabeledField : Name -> Name -> {fmap Name -> Vals} -> Query
   | NestedField : Name -> {fmap Name -> Vals} -> Query -> Query
   | NestedLabeledField : Name -> Name -> {fmap Name -> Vals} -> Query -> Query
-  | InlineFragment : @type Name -> Query -> Query    (* Check it's named type and not list *)
+  | InlineFragment : Name -> Query -> Query    (* Check it's named type and not list *)
   | SelectionSet : Query -> Query -> Query.   (* seq Query but not empty... *)
 
 
@@ -32,6 +36,166 @@ Section Query.
   | ResponseList : ResponseObject -> ResponseObject -> ResponseObject.
 
 
+
+  (* Right now it is returning a GenTree.tree (Name * Name * {fmap Name -> Vals})
+     
+     The tuple represents (label, field name, args) but for the case of unlabeled fields
+     there is some redundancy, where the label is the same as the field name.
+
+     Another option would be to return a GenTree.tree ((Name, {fmap ...}) + (Name, Name, {fmap ...}))
+     but this option doesn't allow (currently) to define Query as ordType, due to sum type
+     not being of ordType itself.
+   *)
+    Fixpoint tree_of_query query : GenTree.tree (Name * Name * {fmap Name -> Vals})  :=
+    match query with
+    | SingleField name args => GenTree.Node 0 [:: GenTree.Leaf (name, name, args)]
+    | LabeledField label name args => GenTree.Node 1 [:: GenTree.Leaf (label, name, args)]
+    | NestedField name args ϕ => GenTree.Node 2 [:: GenTree.Leaf (name, name, args);
+                                                  tree_of_query ϕ]
+    | NestedLabeledField label name args ϕ =>  GenTree.Node 3 [:: GenTree.Leaf (label, name, args);
+                                                                tree_of_query ϕ]
+    | InlineFragment t ϕ => GenTree.Node 4 [:: GenTree.Leaf (t, t, emptym) ;
+                                             tree_of_query ϕ]
+    | SelectionSet ϕ ϕ' => GenTree.Node 5 [:: tree_of_query ϕ ; tree_of_query ϕ']
+    end.
+
+  Fixpoint query_of_tree (tree : GenTree.tree (Name * Name * {fmap Name -> Vals})) : option Query :=
+    match tree with
+    | GenTree.Node 0 [:: GenTree.Leaf (_, name, args)] => Some (SingleField name args)
+    | GenTree.Node 1 [:: GenTree.Leaf (label, name, args)] => Some (LabeledField label name args)
+    | GenTree.Node 2 [:: GenTree.Leaf (_, name, args); t'] =>
+      if (query_of_tree t') is Some q then
+        Some (NestedField name args q)
+      else
+        None
+    | GenTree.Node 3 [:: GenTree.Leaf (label, name, args); t'] =>
+      if (query_of_tree t') is Some q then
+        Some (NestedLabeledField label name args q)
+      else
+        None
+    |  GenTree.Node 4 [:: GenTree.Leaf (_, ty, emptym); t'] =>
+       if (query_of_tree t') is Some q then
+         Some (InlineFragment (NamedType ty) q)
+       else
+         None
+    | GenTree.Node 5 [:: t' ; t''] =>
+      match (query_of_tree t'), (query_of_tree t'') with
+      | Some q, Some q' => Some (SelectionSet q q')
+      | _, _ => None
+      end
+    | _ => None
+    end.
+
+  Lemma pcan_tree_of_query : pcancel tree_of_query query_of_tree.
+  Proof.
+    elim=> //.
+      by move=> s args q /= ->.
+      by move=> l s args q /= ->.
+      by move=> t q /= ->.
+      by move=> q H q' H' /=; rewrite H H'.
+  Qed.
+
+   Definition query_eqMixin := PcanEqMixin pcan_tree_of_query.
+   Canonical query_eqType := EqType Query query_eqMixin.
+   Definition query_choiceMixin := PcanChoiceMixin pcan_tree_of_query.
+   Canonical query_choiceType := ChoiceType Query query_choiceMixin.
+   Definition query_ordMixin := PcanOrdMixin pcan_tree_of_query.
+   Canonical query_ordType := OrdType Query query_ordMixin.
+
+
+
+
+   Fixpoint response_eq r1 r2 :=
+     match r1, r2 with
+     | Empty, Empty => true
+     | Null l, Null l' => l == l'
+     | SingleResult l val, SingleResult l' val' => (l == l') && (val == val')
+     | ListResult l vals, ListResult l' vals' => (l == l') && (vals == vals')
+     | NestedResult l r1', NestedResult l' r2' => (l == l') && (response_eq r1' r2')
+     | NestedListResult l rs, NestedListResult l' rs' =>
+       let fix loop s1 s2 :=
+           match s1, s2 with
+           | [::], [::] => true
+           | r1 :: s1, r2 :: s2 => if response_eq r1 r2 then loop s1 s2 else false
+           | _, _ => false
+           end
+       in
+       (l == l') && loop rs rs'
+     | ResponseList r1' r1'', ResponseList r2' r2'' => (response_eq r1' r2') && (response_eq r1'' r2'')
+     | _, _ => false
+     end.
+
+     
+   (*
+   Fixpoint tree_of_response response : GenTree.tree (Name + (Vals + seq Vals)) :=
+     match response with
+     | Empty => GenTree.Node 0 [::]
+     | Null l => GenTree.Node 1 [:: GenTree.Leaf (inl l)]
+     | SingleResult l val => GenTree.Node 2 [:: GenTree.Leaf (inl l) ; GenTree.Leaf (inr (inl val))]
+     | ListResult l vals => GenTree.Node 3 [:: GenTree.Leaf (inl l) ; GenTree.Leaf (inr (inr vals))]
+     | NestedResult l q => GenTree.Node 4 [:: GenTree.Leaf (inl l) ; tree_of_response q]
+     | NestedListResult l qs => GenTree.Node 5 (GenTree.Leaf (inl l) :: (map tree_of_response qs))
+     | ResponseList q q' => GenTree.Node 6 [:: tree_of_response q ; tree_of_response q']
+     end.
+
+
+   Fixpoint response_of_tree (t : GenTree.tree (Name + (Vals + seq Vals))) :=
+     match t with
+     | GenTree.Node 0 [::] => Empty
+     | GenTree.Node 1 [:: GenTree.Leaf (inl l)] => Null l
+     | GenTree.Node 2 [:: GenTree.Leaf (inl l) ; GenTree.Leaf (inr (inl val))] => SingleResult l val
+     | GenTree.Node 3 [:: GenTree.Leaf (inl l) ; GenTree.Leaf (inr (inr vals))] => ListResult l vals
+     | GenTree.Node 4 [:: GenTree.Leaf (inl l) ; t'] => NestedResult l (response_of_tree t')
+     | GenTree.Node 5 (GenTree.Leaf (inl l) :: t') => NestedListResult l (map response_of_tree t')
+     | GenTree.Node 6 [::  t ; t'] => ResponseList (response_of_tree t) (response_of_tree t')
+     | _ => Empty
+     end.
+
+   Lemma tree_of_responseK : cancel tree_of_response response_of_tree.
+   Proof.
+     elim=> //.
+       by move=> s r /= ->.
+       move=> s rs /=. rewrite map_nseq.
+       
+  Qed. *)
+   
+  (*
+  Fixpoint query_eq q1 q2 :=
+    match q1, q2 with
+    | SingleField name args, SingleField name' args' => (name == name') && (args == args')
+    | LabeledField label name args, LabeledField label' name' args' => (label == label') && (name == name') && (args == args')
+    | NestedField name args ϕ, NestedField name' args' ϕ' => (name == name') && (args == args') && query_eq ϕ ϕ'
+    | NestedLabeledField label name args ϕ, NestedLabeledField label' name' args' ϕ' =>
+      (label == label') && (name == name') && (args == args') && query_eq ϕ ϕ'
+    | InlineFragment t ϕ, InlineFragment t' ϕ' => (t == t') && query_eq ϕ ϕ'
+    | SelectionSet ϕ ϕ', SelectionSet ψ ψ' => (query_eq ϕ ψ) &&  (query_eq ϕ' ψ')
+    | _,  _ => false
+    end.
+
+
+  Lemma query_eqP : Equality.axiom query_eq.
+  Proof.
+    rewrite /Equality.axiom.
+    move=> x y; apply: (iffP idP) => [| <- {y}].
+    move: y; elim: x.
+    by move=> n args; case=> n' args' //=; move/andP=> [/eqP -> /eqP ->].
+    by move=> l n args; case=> l' n' args' //=; move/andP=> [/andP [/eqP -> /eqP ->] /eqP ->].
+    move=> n args q IH; case=> // => n' args' q' /=; move/andP=> [/andP [/eqP -> /eqP ->] H].
+      by apply IH in H; rewrite H.
+    move=> l n args q IH; case=> // => l' n' args' q' /=; move/andP=> [/andP [/andP [/eqP -> /eqP ->] /eqP ->] H].
+      by apply IH in H; rewrite H.
+    move=> t q IH; case=> // => t' q' /=; move/andP=> [/eqP -> H].
+      by apply IH in H; rewrite H.
+    move=> q IH q' IH'. case=> // => q'' q''' //=. move/andP=> [H1 H2].
+    by apply IH in H1; apply IH' in H2; rewrite H1 H2. 
+    elim: x => /=.
+    by move=> s f; rewrite !eqxx.
+    by move=> l s f; rewrite !eqxx.
+    by move=> s f q IH; rewrite !eqxx.
+    by move=> l s f q IH; rewrite !eqxx.
+    by move=> t q IH; rewrite !eqxx.
+    move=> q IH q' IH'. rewrite !eqxx. *)
+    
   Fixpoint isFieldSelection query :=
     match query with
     | SingleField _ _ => true
