src/Example.v
@@ -299,13 +299,11 @@ Section Example.
                                        )
                          ).
 
-    Lemma ev_query_eq_response : eval_query  wf_graph wf_query = query_response.
+    Lemma ev_query_eq_response : response_eq (eval_query  wf_graph wf_query) query_response.
     Proof.
-      rewrite /eval_query /=.
+      move=> /=.
       rewrite /get_target_nodes_with_field /=.
-      rewrite /edges [fset]unlock /=.
-      rewrite /query_response.
-        by [].
+      by rewrite /edges [fset]unlock /=.
     Qed.
     
   End HP.
